code/blake2/Hacl.Blake2s_128.fst
@@ -51,3 +51,5 @@ let store_state128s_to_state32: Core.store_state_st Spec.Blake2S Core.M128 =
   Core.store_state_to_state32 #Spec.Blake2S #Core.M128
 let load_state128s_from_state32: Core.load_state_st Spec.Blake2S Core.M128  =
   Core.load_state_from_state32 #Spec.Blake2S #Core.M128
+
+let blake2s_malloc = Impl.mk_malloc Spec.Blake2S Core.M128
